cp before adding pat type

pulse/pulse2rust/src/ocaml/generated/Pulse2Rust.ml
@@ -938,6 +938,25 @@ and (extract_mlexpr :
                 uu___2::[]);
              FStar_Extraction_ML_Syntax.mlty = uu___3;
              FStar_Extraction_ML_Syntax.loc = uu___4;_},
+           e_r::e_x::uu___5)
+          when
+          let uu___6 = FStar_Extraction_ML_Syntax.string_of_mlpath p in
+          uu___6 = "Pulse.Lib.Reference.replace" ->
+          let uu___6 = extract_mlexpr g e_r in
+          let uu___7 = extract_mlexpr g e_x in
+          Pulse2Rust_Rust_Syntax.mk_mem_replace uu___6 uu___7
+      | FStar_Extraction_ML_Syntax.MLE_App
+          ({
+             FStar_Extraction_ML_Syntax.expr =
+               FStar_Extraction_ML_Syntax.MLE_TApp
+               ({
+                  FStar_Extraction_ML_Syntax.expr =
+                    FStar_Extraction_ML_Syntax.MLE_Name p;
+                  FStar_Extraction_ML_Syntax.mlty = uu___;
+                  FStar_Extraction_ML_Syntax.loc = uu___1;_},
+                uu___2::[]);
+             FStar_Extraction_ML_Syntax.mlty = uu___3;
+             FStar_Extraction_ML_Syntax.loc = uu___4;_},
            e1::[])
           when
           let uu___5 = FStar_Extraction_ML_Syntax.string_of_mlpath p in
@@ -1027,6 +1046,24 @@ and (extract_mlexpr :
           uu___7 = "Pulse.Lib.Mutex.new_mutex" ->
           let e2 = extract_mlexpr g e1 in
           Pulse2Rust_Rust_Syntax.mk_new_mutex e2
+      | FStar_Extraction_ML_Syntax.MLE_App
+          ({
+             FStar_Extraction_ML_Syntax.expr =
+               FStar_Extraction_ML_Syntax.MLE_TApp
+               ({
+                  FStar_Extraction_ML_Syntax.expr =
+                    FStar_Extraction_ML_Syntax.MLE_Name p;
+                  FStar_Extraction_ML_Syntax.mlty = uu___;
+                  FStar_Extraction_ML_Syntax.loc = uu___1;_},
+                uu___2::[]);
+             FStar_Extraction_ML_Syntax.mlty = uu___3;
+             FStar_Extraction_ML_Syntax.loc = uu___4;_},
+           uu___5::e1::uu___6)
+          when
+          let uu___7 = FStar_Extraction_ML_Syntax.string_of_mlpath p in
+          uu___7 = "Pulse.Lib.Mutex.lock" ->
+          let e2 = extract_mlexpr g e1 in
+          Pulse2Rust_Rust_Syntax.mk_lock_mutex e2
       | FStar_Extraction_ML_Syntax.MLE_App
           ({
              FStar_Extraction_ML_Syntax.expr =
@@ -1313,8 +1350,11 @@ and (extract_mlexpr_to_stmts :
                   FStar_Extraction_ML_Syntax.loc = uu___4;_},
                 uu___5)
                when
-               FStar_Compiler_Util.starts_with
-                 (FStar_Pervasives_Native.snd p) "unexplode_ref"
+               (FStar_Compiler_Util.starts_with
+                  (FStar_Pervasives_Native.snd p) "unexplode_ref")
+                 ||
+                 ((FStar_Extraction_ML_Syntax.mlpath_to_string p) =
+                    "Pulse.Lib.Mutex.unlock")
                -> extract_mlexpr_to_stmts g e1
            | uu___ ->
                let uu___1 = lb_init_and_def g lb in
